swap stores at disjoint offsets

mppa_k1c/Asmblockdeps.v
@@ -218,6 +218,12 @@ Proof.
   destruct chunk; simpl; lia.
 Qed.
 
+Remark size_chunk_small: forall chunk,
+    (size_chunk chunk) <= 8.
+Proof.
+  destruct chunk; simpl; lia.
+Qed.
+
 Definition disjoint_chunks
            (ofs1 : offset) (chunk1 : memory_chunk)
            (ofs2 : offset) (chunk2 : memory_chunk) :=
@@ -226,18 +232,20 @@ Definition disjoint_chunks
                 ((Ptrofs.unsigned ofs2),
                  ((Ptrofs.unsigned ofs2) + (size_chunk chunk2))).
 
-(* THIS CANNOT BE PROVED DUE TO OVERFLOW WRAPPING
-(* use something like load_store_other *)
-Lemma store_swap : forall n1 n2 ofs1 ofs2 vs1 vs2 va m0 m0' m1 m2 m1' m2',
+Definition small_offset_threshold := 18446744073709551608.
+
+Lemma store_swap : forall n1 n2 ofs1 ofs2 vs1 vs2 va m0 m1 m2 m1' m2',
     (disjoint_chunks ofs1 (store_chunk n1) ofs2 (store_chunk n2)) ->
+    (Ptrofs.unsigned ofs1) < small_offset_threshold ->
+    (Ptrofs.unsigned ofs2) < small_offset_threshold ->
     store_eval (OStoreRRO n1 ofs1) [vs1; va; Memstate m0] = Some (Memstate m1) ->
     store_eval (OStoreRRO n2 ofs2) [vs2; va; Memstate m1] = Some (Memstate m2) ->
-    store_eval (OStoreRRO n2 ofs2) [vs2; va; Memstate m0'] = Some (Memstate m1') ->
+    store_eval (OStoreRRO n2 ofs2) [vs2; va; Memstate m0] = Some (Memstate m1') ->
     store_eval (OStoreRRO n1 ofs1) [vs1; va; Memstate m1'] = Some (Memstate m2') ->
     m2 = m2'.
 Proof.
   intros until m2'.
-  intros DISJOINT STORE0 STORE1 STORE0' STORE1'.
+  intros DISJOINT SMALL1 SMALL2 STORE0 STORE1 STORE0' STORE1'.
   unfold disjoint_chunks in DISJOINT.
   destruct vs1 as [v1 | ]; simpl in STORE0, STORE1'; try congruence.
   destruct vs2 as [v2 | ]; simpl in STORE1, STORE0'; try congruence.
@@ -261,18 +269,24 @@ Proof.
   rewrite <- E1.
   rewrite <- E1'.
   eapply Mem.store_store_other.
-  {
-    right.
-    pose proof (size_chunk_positive (store_chunk n1)).
-    pose proof (size_chunk_positive (store_chunk n2)).
-    destruct (Intv.range_disjoint _ _ DISJOINT) as [DIS | [DIS | DIS]];
-      unfold Intv.empty in DIS; simpl in DIS.
-    1, 2: lia.
-    destruct (Ptrofs.unsigned_add_either wpofs ofs1) as [R1 | R1]; rewrite R1;
+  2, 3: eassumption.
+
+  right.
+  pose proof (size_chunk_positive (store_chunk n1)).
+  pose proof (size_chunk_positive (store_chunk n2)).
+  pose proof (size_chunk_small (store_chunk n1)).
+  pose proof (size_chunk_small (store_chunk n2)).
+  destruct (Intv.range_disjoint _ _ DISJOINT) as [DIS | [DIS | DIS]];
+    unfold Intv.empty in DIS; simpl in DIS.
+  1, 2: lia.
+  pose proof (Ptrofs.unsigned_range ofs1).
+  pose proof (Ptrofs.unsigned_range ofs2).
+  unfold small_offset_threshold in *.
+  destruct (Ptrofs.unsigned_add_either wpofs ofs1) as [R1 | R1]; rewrite R1;
     destruct (Ptrofs.unsigned_add_either wpofs ofs2) as [R2 | R2]; rewrite R2;
-    try lia.    
-   }
-*)
+      change Ptrofs.modulus with 18446744073709551616 in *; 
+      lia.
+Qed.
 
 Definition goto_label_deps (f: function) (lbl: label) (vpc: val) :=
   match label_pos lbl 0 (fn_blocks f) with
